UBB.Wf.allEq

FreydSSA/BasicBlock/Extrinsic/Basic.lean
@@ -3,7 +3,7 @@ import FreydSSA.Terminator.Extrinsic.Basic
 
 variable {φ ν α} [Φ : InstSet φ (Ty α)] [Φc : CohInstSet φ (Ty α)]
 
-structure UBB.Wf (p : Purity) (Γ : Ctx ν (Ty α)) (β : UBB φ ν κ) (L : LCtx ν (Ty α) κ)
+structure UBB.Wf (p : Purity) (Γ : Ctx ν (Ty α)) (β : UBB φ ν κ) (L : LCtx ν κ (Ty α))
   : Type _ where
   maxTrg : Ctx ν (Ty α)
   body : β.body.WfM p Γ maxTrg
@@ -18,11 +18,19 @@ def UBB.Wf.wk_entry {Γ Δ : Ctx ν (Ty α)} {β : UBB φ ν κ}
     terminator := dβ.terminator.wk_entry w'
   }
 
-def UBB.Wf.wk_exit {L K : LCtx ν (Ty α) κ} {β : UBB φ ν κ}
+def UBB.Wf.wk_exit {L K : LCtx ν κ (Ty α)} {β : UBB φ ν κ}
   (dβ : Wf p Γ β L) (w : L.Wk K) : Wf p Γ β K where
   maxTrg := dβ.maxTrg
   body := dβ.body
   terminator := dβ.terminator.wk_exit w
+
+theorem UBB.Wf.allEq {Γ : Ctx ν (Ty α)} {β : UBB φ ν κ}
+  : (dβ dβ' : UBB.Wf p Γ β L) → dβ = dβ' :=
+  by
+    intro ⟨Γ, db, dt⟩ ⟨Γ', db', dt'⟩
+    cases db.trgEq db'
+    simp only [mk.injEq, heq_eq_eq, true_and]
+    exact ⟨db.allEq db', dt.allEq dt'⟩
 
 def UBody.WfM.compBB {Γ Δ : Ctx ν (Ty α)} {b : UBody φ ν} {β : UBB φ ν κ}
   (db : b.WfM p Γ Δ) (dβ : β.Wf p Δ L) : UBB.Wf p Γ (b.compBB β) L where
